\documentclass{article}
\author{Max Springenberg}
\title{Logik TUT 11}
\usepackage{amsmath}
\usepackage{amssymb}
\usepackage{stmaryrd}
\usepackage{mathtools}
\setcounter{section}{11}

\begin{document}
\maketitle
\newpage

\subsection{Unifikation}
\subsubsection\
$
|L'| = 2\\
A_1 = R(z,f(a))\\
A_2 = R(g(u),u)\\
\\
z_1 = z, z_2 = g\\
\sigma {z \mapsto g(u)}\\
\\
|L'| = 2\\
\\
A_1 = R(g(u),f(a))\\
A_2 = R(g(u),u)\\
z_1 = f(a), z_2 = u\\
\sigma {u \mapsto f(a)}\\
\\
|L'| = 1\\
L'\{R(g(u),f(a))\}\\
$
\subsubsection\
$
|L'| = 2\\
A_1 = Q(b,f(y),h(u))\\
A_2 = R(z,u,h(g(u)))\\
\\
z_1 = b, z_2 = z\\
\sigma {z \mapsto b}\\
\\
|L'| = 2\\
A_1 = Q(b,f(y),h(u))\\
A_2 = R(b,u,h(g(u)))\\
\\
z_1 = f(y), z_2 = u\\
\sigma {u \mapsto f(y)}\\
\\
|L'| = 2\\
A_1 = Q(b,f(y),h(u))\\
A_2 = R(b,f(y),h(g(u)))\\
\\
z_1 = f(u), z_2 = h(g(u))\\
\lightning$ u in f(u)$\\
$
\subsubsection\
$\lightning$ P mit unterschiedlicher Stelligkeit\\
\newpage
\subsection{Unerfuellbarkeit}
$
\begin{matrix*}[l]
        P(c,g(c))                           & x \mapsto c\\
        \neg P(c,g(c)), Q(f(g(c)),g(c))     & y \mapsto g(c), x \mapsto c\\
        \neg Q(f(g(c),g(c)), R(f(g(c)),g(c))& x \mapsto f(g(c))i, z \mapsto g(c)\\
        \neg R(f(g(c)),g(c))                & x,y \mapsto g(c)\\
\end{matrix*}
\\
\\
\begin{matrix*}[l]
        \neg Q(f(g(c),g(c)) &$aus $\neg Q(f(g(c),g(c)), R(f(g(c)),g(c)),    &\neg R(f(g(c)),g(c))\\
        Q(f(g(c)),g(c))     &$aus $\neg P(c,g(c)), Q(f(g(c)),g(c)),         &P(c,g(c))\\
        \Box                &$aus $\neg Q(f(g(c),g(c)),                     &Q(f(g(c)),g(c))\\
\end{matrix*}
$
\newpage
\subsection{Tautalogien}
Annahme Tautalogie, damit $\neg \varphi$ nicht erfuellbar\\
$
\neg \varphi =  \neg \neg(\forall x (P(x) \rightarrow R(f(x))) 
                \land \forall x (R(f(x)) \rightarrow \neg R(x)) 
                \land \exists y(R(y) \land P(y)))\\
\equiv          \forall x (P(x) \rightarrow R(f(x))) 
                \land \forall x (R(f(x)) \rightarrow \neg R(x)) 
                \land \exists y(R(y) \land P(y))\\
\equiv          \forall x (\neg P(x) \lor R(f(x))) 
                \land \forall x (\neg R(f(x)) \lor \neg R(x)) 
                \land \exists y(R(y) \land P(y))\\
\equiv          \forall x((\neg P(x) \lor R(f(x))) \land (\neg R(f(x)) \lor \neg R(x)))
                \land \exists y(R(y) \land P(y))\\
\equiv          \forall x((\neg P(x) \lor R(f(x))) \land (\neg R(f(x)) \lor \neg R(x)))
                \land (R(c) \land P(c))\\
\equiv          \forall x((\neg P(x) \lor R(f(x))) 
                \land (\neg R(f(x)) \lor \neg R(x))
                \land (R(c) \land P(c)))\\
\\
\\
\begin{matrix*}[l]
        \neg P(c) \lor R(f(c))      &x \mapsto c\\
        \neg R(f(c)) \lor \neg R(c) &x \mapsto c\\
\end{matrix*}
\\
\begin{matrix*}[l]
        R(c) \lor R(f(c))   &$aus $R(c) \land P(c))), \neg P(c) \lor R(f(c))\\
        \Box                &$aus $R(c) \lor R(f(c)), \neg R(f(c)) \lor \neg R(c)\\
\end{matrix*}
$
\\
damit Tautalogie\\
\end{document}
